@prefix edsup: <https://github.com/Xachap/EdSup/edsup#> .
@prefix owl: <http://www.w3.org/2002/07/owl#> .
@prefix rdf: <http://www.w3.org/1999/02/22-rdf-syntax-ns#> .
@prefix xml: <http://www.w3.org/XML/1998/namespace> .
@prefix xsd: <http://www.w3.org/2001/XMLSchema#> .
@prefix rdfs: <http://www.w3.org/2000/01/rdf-schema#> .
@base <https://github.com/Xachap/EdSup/edsup> .

<https://github.com/Xachap/EdSup/edsup> rdf:type owl:Ontology ;
                                       <http://purl.org/dc/terms/created> "2019-04-03"^^xsd:date ;
                                       <http://purl.org/dc/terms/creator> _:genid2147483664 ;
                                       <http://purl.org/dc/terms/license> <https://creativecommons.org/licenses/by/4.0/> ;
                                       <http://purl.org/dc/terms/title> "Ontología para la Educación Superior"@es ;
                                       rdfs:comment "Ontología que contiene los elementos más importantes del esquema de conocimiento referente al entorno de la educación superior"@es ;
                                       rdfs:label "Ontología para la Educación Superior"@es ;
                                       owl:versionInfo "0.1" .

#################################################################
#    Annotation properties
#################################################################

###  http://purl.org/dc/terms/created
<http://purl.org/dc/terms/created> rdf:type owl:AnnotationProperty .


###  http://purl.org/dc/terms/creator
<http://purl.org/dc/terms/creator> rdf:type owl:AnnotationProperty .


###  http://purl.org/dc/terms/license
<http://purl.org/dc/terms/license> rdf:type owl:AnnotationProperty .


###  http://purl.org/dc/terms/title
<http://purl.org/dc/terms/title> rdf:type owl:AnnotationProperty .


###  http://www.w3.org/2002/07/owl#cardinality
owl:cardinality rdf:type owl:AnnotationProperty .


###  http://xmlns.com/foaf/0.1/mbox
<http://xmlns.com/foaf/0.1/mbox> rdf:type owl:AnnotationProperty .


###  http://xmlns.com/foaf/0.1/name
<http://xmlns.com/foaf/0.1/name> rdf:type owl:AnnotationProperty .


#################################################################
#    Object Properties
#################################################################

###  https://github.com/Xachap/EdSup/edsup#asignaturaEstudiadaPor
:asignaturaEstudiadaPor rdf:type owl:ObjectProperty ;
                        owl:inverseOf :estudiaAsignatura ;
                        rdfs:domain :Asignatura ;
                        rdfs:range :Alumno ;
                        rdfs:comment "Relaciona una asignatura con sus alumnos."@es ,
                                     "Relates a subject to its students."@en ;
                        rdfs:label "Asignatura estudiada por"@es ,
                                   "Subject learned by"@en .


###  https://github.com/Xachap/EdSup/edsup#asignaturaImpartidaPor
:asignaturaImpartidaPor rdf:type owl:ObjectProperty ;
                        rdfs:domain :Asignatura ;
                        rdfs:range :Profesor ;
                        rdfs:comment "Relaciona una asignatura con un profesor."@es ,
                                     "Relates a subject with a teacher."@en ;
                        rdfs:label "Asignatura impartida por"@es ,
                                   "Subject teached by"@en .


###  https://github.com/Xachap/EdSup/edsup#competenciaEnAsignatura
:competenciaEnAsignatura rdf:type owl:ObjectProperty ;
                         owl:inverseOf :tieneCompetencia ;
                         rdfs:domain :Competencia ;
                         rdfs:range :Asignatura ;
                         rdfs:comment "Relaciona una asignatura con una competencia."@es ,
                                      "Relates a subject with a competence."@en ;
                         rdfs:label "Competence in subject"@en ,
                                    "Competencia en asignatura"@es .


###  https://github.com/Xachap/EdSup/edsup#coordinaCurso
:coordinaCurso rdf:type owl:ObjectProperty ;
               owl:inverseOf :cursoCoordinado ;
               rdfs:domain :Coordinador ;
               rdfs:range :Curso ;
               rdfs:comment "Relaciona un coordinador con el curso que dirige."@es ,
                            "Relates a coordinator with their corresponding course."@en ;
               rdfs:label "Coordina curso"@es ,
                          "Coordinates course"@en .


###  https://github.com/Xachap/EdSup/edsup#cursoCoordinado
:cursoCoordinado rdf:type owl:ObjectProperty ;
                 rdfs:domain :Curso ;
                 rdfs:range :Coordinador ;
                 rdfs:comment "Relaciona un curso con un coordinador."@es ,
                              "Relates a course with a coordinator."@en ;
                 rdfs:label "Coordinated course"@en ,
                            "Curso coordinado"@es .


###  https://github.com/Xachap/EdSup/edsup#dirigeEscuela
:dirigeEscuela rdf:type owl:ObjectProperty ;
               owl:inverseOf :escuelaDirigida ;
               rdfs:domain :Director ;
               rdfs:range :Escuela ;
               rdfs:comment "Relaciona un director con la escuela en la que ocupa dicho cargo."@es ,
                            "Relates a director with its school."@en ;
               rdfs:label "Dirige escuela"@es ,
                          "Heads up school"@en .


###  https://github.com/Xachap/EdSup/edsup#escuelaDirigida
:escuelaDirigida rdf:type owl:ObjectProperty ;
                 rdfs:domain :Escuela ;
                 rdfs:range :Director ;
                 rdfs:comment "Relaciona una escuela con su director."@es ,
                              "Relates a school with its director."@en ;
                 rdfs:label "Directed school"@en ,
                            "Escuela dirigida"@es .


###  https://github.com/Xachap/EdSup/edsup#estudiaAsignatura
:estudiaAsignatura rdf:type owl:ObjectProperty ;
                   rdfs:domain :Alumno ;
                   rdfs:range :Asignatura ;
                   rdfs:comment "Relaciona un alumno con una de las asignaturas en las que está inscrito."@es ,
                                "Relates a student with a subject in which is enrolled."@en ;
                   rdfs:label "Estudia asignatura"@es ,
                              "Learns subject"@en .


###  https://github.com/Xachap/EdSup/edsup#evaluacionEnAsignatura
:evaluacionEnAsignatura rdf:type owl:ObjectProperty ;
                        rdfs:domain :Evaluacion ;
                        rdfs:range :Asignatura ;
                        rdfs:comment "Relaciona una asignatura con una instancia de método de evaluación."@es ,
                                     "Relates a subject with an instance of evaluation method."@en ;
                        rdfs:label "Evaluation method in subject"@en ,
                                   "Sistema de evaluación en asignatura"@es .


###  https://github.com/Xachap/EdSup/edsup#imparteAsignatura
:imparteAsignatura rdf:type owl:ObjectProperty ;
                   owl:inverseOf :asignaturaImpartidaPor ;
                   rdfs:domain :Profesor ;
                   rdfs:range :Asignatura ;
                   rdfs:comment "Relaciona un profesor con una asignatura en la que imparte clase."@es ,
                                "Relates a teacher with a subject in which teaches."@en ;
                   rdfs:label "Imparte asignatura"@es ,
                              "Teaches subject"@en .


###  https://github.com/Xachap/EdSup/edsup#impartidoEn
:impartidoEn rdf:type owl:ObjectProperty ;
             rdfs:domain :Titulo ;
             rdfs:range :Escuela ;
             rdfs:comment "Relaciona una escuela con un título."@es ,
                          "Relates a school with a certificate."@en ;
             rdfs:label "Impartido en"@es ,
                        "Teached in"@en .


###  https://github.com/Xachap/EdSup/edsup#materialEnAsignatura
:materialEnAsignatura rdf:type owl:ObjectProperty ;
                      rdfs:domain :Material ;
                      rdfs:range :Asignatura ;
                      rdfs:comment "Relaciona una asignatura con una instancia de material didáctico."@es ,
                                   "Relates a subject with an instance of didactic material."@en ;
                      rdfs:label "Material en asignatura"@es ,
                                 "Material in subject"@en .


###  https://github.com/Xachap/EdSup/edsup#perteneceACurso
:perteneceACurso rdf:type owl:ObjectProperty ;
                 rdfs:domain :Semestre ;
                 rdfs:range :Curso ;
                 rdfs:comment "Relaciona un curso con un semestre específico."@es ,
                              "Relates course with a specific semester."@en ;
                 rdfs:label "Belongs to course"@en ,
                            "Pertenece a curso"@es .


###  https://github.com/Xachap/EdSup/edsup#perteneceADoctorado
:perteneceADoctorado rdf:type owl:ObjectProperty ;
                     rdfs:domain :Tesis ;
                     rdfs:range :Doctorado ;
                     rdfs:comment "Relaciona un programa de doctorado con su tesis."@es ,
                                  "Relates a doctorate program with its thesis."@en ;
                     rdfs:label "Belongs to doctorate"@en ,
                                "Pertenece a doctorado"@es .


###  https://github.com/Xachap/EdSup/edsup#perteneceASemestre
:perteneceASemestre rdf:type owl:ObjectProperty ;
                    owl:inverseOf :tieneAsignatura ;
                    rdfs:domain :Asignatura ;
                    rdfs:range :Semestre ;
                    rdfs:comment "Relaciona un semestre con uns asignatura."@es ,
                                 "Relates a semester with a subject."@en ;
                    rdfs:label "Belongs to semester"@en ,
                               "Pertenece a semestre"@es .


###  https://github.com/Xachap/EdSup/edsup#perteneceATitulo
:perteneceATitulo rdf:type owl:ObjectProperty ;
                  rdfs:domain :Curso ;
                  rdfs:range :Titulo ;
                  rdfs:comment "Relaciona un título con un curso."@es ,
                               "Relates a course with a certificate."@en ;
                  rdfs:label "Belongs to certificate"@en ,
                             "Pertenece a título"@es .


###  https://github.com/Xachap/EdSup/edsup#perteneceAUniversidad
:perteneceAUniversidad rdf:type owl:ObjectProperty ;
                       owl:inverseOf :tieneEscuela ;
                       rdfs:domain :Escuela ;
                       rdfs:range :Universidad ;
                       rdfs:comment "Relaciona una Universidad con una escuela determinada."@es ,
                                    "Relates a University with a certain school."@en ;
                       rdfs:label "Belongs to University"@en ,
                                  "PerteneceAUniversidad"@es .


###  https://github.com/Xachap/EdSup/edsup#tareaEnDoctorado
:tareaEnDoctorado rdf:type owl:ObjectProperty ;
                  owl:inverseOf :tieneTareaInvestigacion ;
                  rdfs:domain :Tarea_investigacion ;
                  rdfs:range :Doctorado ;
                  rdfs:comment "Relaciona un programa de doctorado con una instancia de tarea de investigación."@es ,
                               "Relates a doctorate program with an instance of research task."@en ;
                  rdfs:label "Tarea en doctorado"@es ,
                             "Task in doctorate"@en .


###  https://github.com/Xachap/EdSup/edsup#tieneAsignatura
:tieneAsignatura rdf:type owl:ObjectProperty ;
                 rdfs:domain :Semestre ;
                 rdfs:range :Asignatura ;
                 rdfs:comment "Relaciona una asignatura con un semestre que la contiene."@es ,
                              "Relates a subject with its semester."@en ;
                 rdfs:label "Has subject"@en ,
                            "Tiene asignatura"@es .


###  https://github.com/Xachap/EdSup/edsup#tieneCompetencia
:tieneCompetencia rdf:type owl:ObjectProperty ;
                  rdfs:domain :Asignatura ;
                  rdfs:range :Competencia ;
                  rdfs:comment "Relaciona una competencia determinada con una asignatura."@es ,
                               "Relates a competence with a subject."@en ;
                  rdfs:label "Has competence"@en ,
                             "Tiene competencia"@es .


###  https://github.com/Xachap/EdSup/edsup#tieneCurso
:tieneCurso rdf:type owl:ObjectProperty ;
            owl:inverseOf :perteneceATitulo ;
            rdfs:domain :Titulo ;
            rdfs:range :Curso ;
            rdfs:comment "Relaciona cada curso con el título al que pertenece."@es ,
                         "Relates a course with their corresponding certificate."@en ;
            rdfs:label "Has course"@en ,
                       "Tiene curso"@es .


###  https://github.com/Xachap/EdSup/edsup#tieneEscuela
:tieneEscuela rdf:type owl:ObjectProperty ;
              rdfs:domain :Universidad ;
              rdfs:range :Escuela ;
              rdfs:comment "Relaciona una escuela con la Universidad a la que pertenece."@es ,
                           "Relates a school with the University that it belongs."@en ;
              rdfs:label "Has school"@en ,
                         "Tiene escuela"@es .


###  https://github.com/Xachap/EdSup/edsup#tieneMaterial
:tieneMaterial rdf:type owl:ObjectProperty ;
               owl:inverseOf :materialEnAsignatura ;
               rdfs:domain :Asignatura ;
               rdfs:range :Material ;
               rdfs:comment "Relaciona una instancia de material didáctico con la asignatura en la que se usa."@es ,
                            "Relates an instance of didactic material with a certain subject."@en ;
               rdfs:label "Has material"@en ,
                          "Tiene material"@es .


###  https://github.com/Xachap/EdSup/edsup#tieneSemestre
:tieneSemestre rdf:type owl:ObjectProperty ;
               owl:inverseOf :perteneceACurso ;
               rdfs:domain :Curso ;
               rdfs:range :Semestre ;
               rdfs:comment "Relaciona un semestre con el curso al que pertenece."@es ,
                            "Relates a specific semester with a certain course."@en ;
               rdfs:label "Has semester"@en ,
                          "Tiene semestre"@es .


###  https://github.com/Xachap/EdSup/edsup#tieneSistemaEvaluacion
:tieneSistemaEvaluacion rdf:type owl:ObjectProperty ;
                        owl:inverseOf :evaluacionEnAsignatura ;
                        rdfs:domain :Asignatura ;
                        rdfs:range :Evaluacion ;
                        rdfs:comment "Relaciona una instancia de método de evaluación con la asignatura en la que se utiliza."@es ,
                                     "Relates an instance of evaluation method with the subject in which it is used."@en ;
                        rdfs:label "Has evaluation method"@en ,
                                   "Tiene sistema de evaluación"@es .


###  https://github.com/Xachap/EdSup/edsup#tieneTareaInvestigacion
:tieneTareaInvestigacion rdf:type owl:ObjectProperty ;
                         rdfs:domain :Doctorado ;
                         rdfs:range :Tarea_investigacion ;
                         rdfs:comment "Relaciona una instancia de tarea de investigación con el doctorado en el que se desarrolla."@es ,
                                      "Relates an instance of research task with the doctorate program in which is being performed."@en ;
                         rdfs:label "Has research task"@en ,
                                    "Tiene tarea de investigación"@es .


###  https://github.com/Xachap/EdSup/edsup#tieneTesis
:tieneTesis rdf:type owl:ObjectProperty ;
            owl:inverseOf :perteneceADoctorado ;
            rdfs:domain :Doctorado ;
            rdfs:range :Tesis ;
            rdfs:comment "Relaciona una tesis con un programa de doctorado al que pertenece."@es ,
                         "Relates a thesis with a doctorate program."@en ;
            rdfs:label "Has Thesis"@en ,
                       "Tiene Tesis"@es .


###  https://github.com/Xachap/EdSup/edsup#tieneTitulo
:tieneTitulo rdf:type owl:ObjectProperty ;
             owl:inverseOf :impartidoEn ;
             rdfs:domain :Escuela ;
             rdfs:range :Titulo ;
             rdfs:comment "Relaciona un título con la escuela en la que se imparte."@es ,
                          "Relates a degree with a school in which is carried out."@en ;
             rdfs:label "Has degree"@en ,
                        "Tiene Título"@es .


#################################################################
#    Data properties
#################################################################

###  https://github.com/Xachap/EdSup/edsup#num_creditos
:num_creditos rdf:type owl:DatatypeProperty ;
              rdfs:domain :Asignatura ;
              rdfs:range xsd:double ;
              rdfs:comment "Indica el número de créditos que tiene una asignatura."@es ,
                           "Number of credits that a subject has."@en ;
              rdfs:label "Number of credits"@en ,
                         "Numero de créditos"@es .


#################################################################
#    Classes
#################################################################

###  http://org.semanticweb.owlapi/error#Error2
<http://org.semanticweb.owlapi/error#Error2> rdf:type owl:Class .


###  https://github.com/Xachap/EdSup/edsup#Alumno
:Alumno rdf:type owl:Class ;
        rdfs:subClassOf <http://xmlns.com/foaf/0.1/Person> ;
        rdfs:comment "Agent enrolled in several subjects, who seeks to obtain the fixed competences of a particular degree."@en ,
                     "Agente inscrito en varias asignaturas, que busca obtener las competencias fijadas de un título en concreto"@es ;
        rdfs:label "Alumno"@es ,
                   "Student"@en .


###  https://github.com/Xachap/EdSup/edsup#Asignatura
:Asignatura rdf:type owl:Class ;
            rdfs:subClassOf <http://xmlns.com/foaf/0.1/Group> ;
            rdfs:comment "Part of a semester, where a set of knowledge, that come specified in the competences, is teached. They use two different type of resources: didactic material and evaluation methods. Their duration is fixed by the number of credits."@en ,
                         "Parte de un semestre, donde se imparten una serie de conocimientos que vienen especificados en las competencias. Usan dos recursos bien diferenciados que son el material educativo y los sistemas de evaluación. Su duración viene fijada por el número de créditos."@es ;
            rdfs:label "Asignatura"@es ,
                       "Subject"@en .


###  https://github.com/Xachap/EdSup/edsup#Competencia
:Competencia rdf:type owl:Class ;
             rdfs:subClassOf owl:Thing ;
             rdfs:comment "Habilidades y/o conocimientos que el título debe reflejar. Se imparten en una o varias asignaturas."@es ,
                          "Skills and/or knowledge that the title should attest. They are taught in one or several subjects."@en ;
             rdfs:label "Competencia"@es ,
                        "Competency"@en .


###  https://github.com/Xachap/EdSup/edsup#Coordinador
:Coordinador rdf:type owl:Class ;
             rdfs:subClassOf :Profesor ;
             rdfs:comment "Profesor que además tiene la obligación de asegurar el correcto funcionamiento de un determinado curso."@es ,
                          "Teacher who also has to ensure the proper functioning of a particular course."@en ;
             rdfs:label "Coordinador"@es ,
                        "Coordinator"@en .


###  https://github.com/Xachap/EdSup/edsup#Curso
:Curso rdf:type owl:Class ;
       rdfs:subClassOf owl:Thing ;
       rdfs:comment "First temporal division of first and second cycle degrees. Corresponds to one year."@en ,
                    "Primera división temporal de los títulos de primer y segundo ciclo. Corresponde a un año."@es ;
       rdfs:label "Course"@en ,
                  "Curso"@es .


###  https://github.com/Xachap/EdSup/edsup#Director
:Director rdf:type owl:Class ;
          rdfs:subClassOf :Profesor ;
          rdfs:comment "Profesor que además tiene la obligación de asegurar el correcto funcionamiento de la escuela."@es ,
                       "Teacher who also has to ensure the proper functioning of a school."@en ;
          rdfs:label "Director"@en ,
                     "Director"@es .


###  https://github.com/Xachap/EdSup/edsup#Doctorado
:Doctorado rdf:type owl:Class ;
           rdfs:subClassOf :Titulo ;
           owl:disjointWith <https://github.com/Xachap/EdSup/edsup#1_2_ciclo> ;
           rdfs:comment "Third cycle degree that has a special structure respect to the 1st and 2nd cycle, so it composes a different subclass."@en ,
                        "Título de tercer ciclo que tiene una estructura especial respecto a los de 1º y 2º ciclo, por lo que compone otra subclase diferente"@es ;
           rdfs:label "Doctorado"@es ,
                      "Doctoral degree"@en .


###  https://github.com/Xachap/EdSup/edsup#Escuela
:Escuela rdf:type owl:Class ;
         rdfs:subClassOf <http://www.w3.org/ns/org#Organization> ;
         rdfs:comment "A place where a number of specific degrees are taught."@en ,
                      "Lugar donde se imparten una serie de títulos determinados."@es ;
         rdfs:label "Escuela"@es ,
                    "School"@en .


###  https://github.com/Xachap/EdSup/edsup#Evaluacion
:Evaluacion rdf:type owl:Class ;
            rdfs:subClassOf owl:Thing ;
            rdfs:comment "A method or set of methods that ensures that the student has achieved the proposed competencies."@en ,
                         "Método o conjunto de métodos que permite asegurar que el alumno ha conseguido las competencias propuestas"@es ;
            rdfs:label "Evaluacion"@es ,
                       "Evaluation"@en .


###  https://github.com/Xachap/EdSup/edsup#Grado
:Grado rdf:type owl:Class ;
       rdfs:subClassOf <https://github.com/Xachap/EdSup/edsup#1_2_ciclo> ;
       owl:disjointWith :Master ;
       rdfs:comment "First cycle degree, corresponds to the lowest educational step within higher education."@en ,
                    "Título de primer ciclo, corresponde a la formación más baja dentro de la educación superior."@es ;
       rdfs:label "Degree"@en ,
                  "Grado"@es .


###  https://github.com/Xachap/EdSup/edsup#Master
:Master rdf:type owl:Class ;
        rdfs:subClassOf <https://github.com/Xachap/EdSup/edsup#1_2_ciclo> ;
        rdfs:comment "Second cycle degree, with a duration shorter than that a Degree."@en ,
                     "Título de segundo ciclo, con duración inferior a la del Grado."@es ;
        rdfs:label "Bachelor's degree"@en ,
                   "Máster"@es .


###  https://github.com/Xachap/EdSup/edsup#Material
:Material rdf:type owl:Class ;
          rdfs:subClassOf owl:Thing ;
          rdfs:comment "Any resource that is provided to the student to develop a series of fixed competences."@en ,
                       "Todo recurso que se le proporciona al alumno para que desarrolle una serie de competencias fijadas."@es ;
          rdfs:label "Didactic material"@en ,
                     "Material didáctico"@es .


###  https://github.com/Xachap/EdSup/edsup#Profesor
:Profesor rdf:type owl:Class ;
          rdfs:subClassOf <http://xmlns.com/foaf/0.1/Person> ;
          rdfs:comment "Agent in charge of providing educational material and evaluating students in one or more subjects."@en ,
                       "Agente encargado de proporcionar material educativo y evaluar a los alumnos de una o varias asignaturas."@es ;
          rdfs:label "Profesor"@es ,
                     "Teacher"@en .


###  https://github.com/Xachap/EdSup/edsup#Semestre
:Semestre rdf:type owl:Class ;
          rdfs:subClassOf <http://org.semanticweb.owlapi/error#Error2> ,
                          owl:Thing ;
          rdfs:comment "Second temporal division of first and second cycle degrees. Each course corresponds to two semesters."@en ,
                       "Segunda división temporal de los títulos de primer y segundo ciclo. A cada curso le corresponde dos semestres."@es ;
          rdfs:label "Semester"@en ,
                     "Semestre"@es .


###  https://github.com/Xachap/EdSup/edsup#Tarea_investigacion
:Tarea_investigacion rdf:type owl:Class ;
                     rdfs:subClassOf owl:Thing ;
                     rdfs:comment "Actividades a realizar a lo largo de un doctorado que están relacionadas con la tesis."@es ,
                                  "Task to be carried out during a doctorate that are related to the thesis."@en ;
                     rdfs:label "Research task"@en ,
                                "Tarea de investigacion"@es .


###  https://github.com/Xachap/EdSup/edsup#Tesis
:Tesis rdf:type owl:Class ;
       rdfs:subClassOf owl:Thing ;
       rdfs:comment "Trabajo que se realiza a lo largo de un doctorado, en el que se investiga sobre un tema en concreto para sacar conclusiones y resultados de utilidad."@es ,
                    "Work carried out during a doctorate, in which a research is carried out on a specific subject in order to draw conclusions and useful results."@en ;
       rdfs:label "Tesis"@es ,
                  "Thesis"@en .


###  https://github.com/Xachap/EdSup/edsup#Titulo
:Titulo rdf:type owl:Class ;
        rdfs:subClassOf owl:Thing ;
        rdfs:comment "Academic itinerary where a series of concepts are taught. If the evaluation of these concepts is positive, the student obtains the certificate of degree."@en ,
                     "Itinerario académico donde se imparten una serie de conceptos. Si la evaluación de estos conceptos es positiva, el alumno obtiene el certificado de título."@es ;
        rdfs:label "Certificate"@en ,
                   "Título"@es .


###  https://github.com/Xachap/EdSup/edsup#Universidad
:Universidad rdf:type owl:Class ;
             rdfs:subClassOf <http://www.w3.org/ns/org#Organization> ;
             rdfs:comment "Institución donde se imparten cada uno de los títulos de educación superior."@es ,
                          "Institution where each of the higher education degrees are taught."@en ;
             rdfs:label "Universidad"@es ,
                        "University"@en .


###  https://github.com/Xachap/EdSup/edsup#1_2_ciclo
<https://github.com/Xachap/EdSup/edsup#1_2_ciclo> rdf:type owl:Class ;
                                                rdfs:subClassOf :Titulo ;
                                                rdfs:comment "Bachelor's and Master's degrees (subclass). They have in common their structure, since both are composed of a series of subjects encapsulated in courses and semesters."@en ,
                                                             "Títulos de grado y máster (subclase). Tienen en común su estructura, ya que ambos se componen de una serie de asignaturas encapsuladas en cursos y semestres."@es ;
                                                rdfs:label "1_2_ciclo"@es ,
                                                           "1_2_cycle"@en .


###  http://www.w3.org/ns/org#Organization
<http://www.w3.org/ns/org#Organization> rdf:type owl:Class .


###  http://xmlns.com/foaf/0.1/Group
<http://xmlns.com/foaf/0.1/Group> rdf:type owl:Class .


###  http://xmlns.com/foaf/0.1/Person
<http://xmlns.com/foaf/0.1/Person> rdf:type owl:Class .


_:genid1 <http://xmlns.com/foaf/0.1/mbox> "j.perezmar@posgrado.uimp.es" ;
         <http://xmlns.com/foaf/0.1/name> "Jesús Pérez" .

[ owl:cardinality "2"^^xsd:int
 ] .

###  Generated by the OWL API (version 5.1.9) https://github.com/owlcs/owlapi/
